\documentclass{article}

\usepackage[letterpaper, margin=1in, headheight=15pt]{geometry}
\usepackage{amsmath,amssymb}
\setlength{\parindent}{4pt}

\newcommand{\diedie}[2]{\frac{\partial #1}{\partial #2}}
\let\die\partial
\newcommand{\christoffel}[2]{\genfrac{\{}{\}}{0pt}{}{#1}{#2}}
\newcommand{\Q}{{\vphantom{-1}}}

\begin{document}

We begin with a 3 point rank-2 integral

\begin{equation}
	\int_l \frac{l^{\mu 1}\; l^{\mu 2}}{[l^2 -m^2][(l+k_1)^2 -m^2][(l+k_2)^2 -m^2]}
\end{equation}
Performing Feynman parametrization
\begin{equation}
	 \int_0^1 dx dy \int_l \frac{l^{\mu 1}l^{\mu 2}}{[l^2+2l.k_1 x + 2l.k_2 y - m^2]^3}
\end{equation}
Adding $k_1.k_1x^2=0$ , $k_2.k_2y^2=0$ and $k_1.k_2 xy - k_1.k_2 xy = 0$ we have:
\begin{align}
	&= \int_0^1 dx dy \int_l \frac{l^{\mu 1}l^{\mu 2}}{[(l+k_1 x+k_2 y)^2 -k_1.k_2 xy - m^2]^3}\\
	&= \int_0^1 dx dy \int_l \frac{(l-2k_1x-2k_2y)^{\mu 1}(l-2k_1x-2k_2y)^{\mu 2}}{[l^2- 2k_1.k_2xy -m^2]^3}
\end{align}

\end{document}
